<?xml version="1.0"?>
<rdf:RDF xmlns="http://purl.enanomapper.net/onto/internal/bfo-ext.owl#"
     xml:base="http://purl.enanomapper.net/onto/internal/bfo-ext.owl"
     xmlns:rdf="http://www.w3.org/1999/02/22-rdf-syntax-ns#"
     xmlns:owl="http://www.w3.org/2002/07/owl#"
     xmlns:xml="http://www.w3.org/XML/1998/namespace"
     xmlns:xsd="http://www.w3.org/2001/XMLSchema#"
     xmlns:rdfs="http://www.w3.org/2000/01/rdf-schema#"
     xmlns:obo="http://purl.obolibrary.org/obo/"
     xmlns:dc="http://purl.org/dc/elements/1.1/">

    <owl:Ontology rdf:about="http://enanomapper.github.io/ontologies/internal/bfo-ext.owl">
        <dc:contributor>Laurent Winckers</dc:contributor>
	<dc:license>CC-BY 4.0 https://creativecommons.org/licenses/by/4.0/</dc:license>
	<rdfs:comment>This ontology contains proposed extensions to the Basic Formal ON, which in due course will be submitted to the BFO. </rdfs:comment>
    </owl:Ontology>

    <!-- http://purl.enanomapper.org/onto/ENM_0000107 -->

    <owl:Class rdf:about="http://purl.enanomapper.org/onto/ENM_0000107">
        <rdfs:subClassOf rdf:resource="http://purl.obolibrary.org/obo/BFO_0000019"/>
        <rdfs:label xml:lang="en">Preferential orientation</rdfs:label>
    </owl:Class>

    <!-- http://purl.enanomapper.org/onto/ENM_0000103 -->

    <owl:Class rdf:about="http://purl.enanomapper.org/onto/ENM_0000103">
        <rdfs:subClassOf rdf:resource="http://purl.obolibrary.org/obo/BFO_0000019"/>
        <rdfs:label xml:lang="en">osmotic concentration</rdfs:label>
    </owl:Class>

    <!-- http://purl.enanomapper.org/onto/ENM_0000101 -->

    <owl:Class rdf:about="http://purl.enanomapper.org/onto/ENM_0000101">
        <rdfs:subClassOf rdf:resource="http://purl.obolibrary.org/obo/BFO_0000019"/>
        <rdfs:label xml:lang="en">redox speciation</rdfs:label>
    </owl:Class>
    
    <owl:Class rdf:about="http://purl.enanomapper.org/onto/ENM_0000114">
  	<rdfs:subClassOf rdf:resource="http://purl.obolibrary.org/obo/BFO_0000015"/>
  	<obo:IAO_0000115>The evolutionary process by which populations evolve to become distinct species.</obo:IAO_0000115>
  	<rdfs:label xml:lang="en">Speciation</rdfs:label>
    </owl:Class>



    <!-- http://purl.enanomapper.org/onto/ENM_9000003 -->

    <owl:Class rdf:about="http://purl.enanomapper.org/onto/ENM_9000003">
        <rdfs:subClassOf rdf:resource="http://purl.obolibrary.org/obo/BFO_0000019"/>
        <obo:IAO_0000115>The propensity of a powder to become aerosolised by mechanical agitation. The dustiness of a particular sample is very dependent on its moisture content and static electrical properties. </obo:IAO_0000115>
        <obo:IAO_0000119>RSC technical brief on nanomaterial characterization</obo:IAO_0000119>
        <rdfs:label xml:lang="en">dustiness</rdfs:label>
    </owl:Class>
    


    <!-- http://purl.enanomapper.org/onto/ENM_9000004 -->

    <owl:Class rdf:about="http://purl.enanomapper.org/onto/ENM_9000004">
        <rdfs:subClassOf rdf:resource="http://purl.obolibrary.org/obo/BFO_0000019"/>
        <obo:IAO_0000115>Pour density requires the weighing of a known volume of freshly poured powder.</obo:IAO_0000115>
        <obo:IAO_0000119>RSC technical brief on nanomaterial characterization</obo:IAO_0000119>
        <rdfs:label xml:lang="en">pour density</rdfs:label>
    </owl:Class>
    



    <!-- http://purl.enanomapper.org/onto/ENM_9000100 -->

    <owl:Class rdf:about="http://purl.enanomapper.org/onto/ENM_9000100">
        <rdfs:subClassOf rdf:resource="http://purl.obolibrary.org/obo/BFO_0000019"/>
        <obo:IAO_0000115 xml:lang="en">The boiling point of a substance is the temperature at which the vapor pressure of the liquid equals the pressure surrounding the liquid and the liquid changes into a vapor. The boiling point of a liquid varies depending upon the surrounding environmental pressure.</obo:IAO_0000115>
        <rdfs:label xml:lang="en">boiling point</rdfs:label>
    </owl:Class>
    


</rdf:RDF>
